SCP-2499 - Remove contract comparison from Isabelle semantics and update proofs

isabelle/MoneyPreservation.thy
@@ -42,7 +42,7 @@ lemma moneyInPayments_works_on_rev : "moneyInPayments payments = moneyInPayments
   using moneyInPayments_rev_cons by auto
 
 fun moneyInReduceResult :: "Payment list \<Rightarrow> State \<Rightarrow> ReduceResult \<Rightarrow> int" where
-"moneyInReduceResult pa sta (ContractQuiescent wa newPa newSta cont) = moneyInState newSta + moneyInPayments newPa" |
+"moneyInReduceResult pa sta (ContractQuiescent newReduced wa newPa newSta cont) = moneyInState newSta + moneyInPayments newPa" |
 "moneyInReduceResult pa sta RRAmbiguousSlotIntervalError = moneyInState sta + moneyInPayments pa"
 
 fun moneyInInput :: "Input \<Rightarrow> int" where
@@ -62,7 +62,7 @@ fun moneyInApplyResult :: "State \<Rightarrow> Input \<Rightarrow> ApplyResult \
 "moneyInApplyResult state inp ApplyNoMatchError = moneyInState state + moneyInInput inp"
 
 fun moneyInApplyAllResult :: "State \<Rightarrow> Input list \<Rightarrow> Payment list \<Rightarrow> ApplyAllResult \<Rightarrow> int" where
-"moneyInApplyAllResult state inps pa (ApplyAllSuccess newWa newPa newSta newCont) =
+"moneyInApplyAllResult state inps pa (ApplyAllSuccess newReduced newWa newPa newSta newCont) =
   moneyInState newSta + moneyInPayments newPa" |
 "moneyInApplyAllResult state inps pa ApplyAllNoMatchError =
   moneyInState state + moneyInInputs inps + moneyInPayments pa" |
@@ -427,19 +427,19 @@ lemma reductionLoop_preserves_money_NoPayment_not_ReduceNoWarning :
   "warning \<noteq> ReduceNoWarning \<Longrightarrow>
    x = warning # warnings \<Longrightarrow>
    (validAndPositive_state newState \<Longrightarrow>
-    moneyInState newState + moneyInPayments payments = moneyInReduceResult xa newState (reductionLoop env newState ncontract x xa)) \<Longrightarrow>
+    moneyInState newState + moneyInPayments payments = moneyInReduceResult xa newState (reductionLoop reduced env newState ncontract x xa)) \<Longrightarrow>
     validAndPositive_state state \<Longrightarrow>
     reduceContractStep env state contract = Reduced warning ReduceNoPayment newState ncontract \<Longrightarrow>
-    moneyInState state + moneyInPayments payments = moneyInReduceResult payments state (reductionLoop env newState ncontract x xa)"
+    moneyInState state + moneyInPayments payments = moneyInReduceResult payments state (reductionLoop reduced env newState ncontract x xa)"
   by (metis ReduceResult.exhaust add.left_neutral moneyInReduceEffect.simps(2) moneyInReduceResult.simps(1) moneyInReduceResult.simps(2) moneyInReduceStepResult.simps(1) reduceContractStep_preserves_money reduceContractStep_preserves_validAndPositive_state)
 
 lemma reductionLoop_preserves_money_NoPayment :
   "x = (if warning = ReduceNoWarning then warnings else warning # warnings) \<Longrightarrow>
    (validAndPositive_state newState \<Longrightarrow>
-    moneyInState newState + moneyInPayments payments = moneyInReduceResult xa newState (reductionLoop env newState ncontract x xa)) \<Longrightarrow>
+    moneyInState newState + moneyInPayments payments = moneyInReduceResult xa newState (reductionLoop reduced env newState ncontract x xa)) \<Longrightarrow>
     validAndPositive_state state \<Longrightarrow>
     reduceContractStep env state contract = Reduced warning ReduceNoPayment newState ncontract \<Longrightarrow>
-    moneyInState state + moneyInPayments payments = moneyInReduceResult payments state (reductionLoop env newState ncontract x xa)"
+    moneyInState state + moneyInPayments payments = moneyInReduceResult payments state (reductionLoop reduced env newState ncontract x xa)"
   by (metis ReduceResult.exhaust add.left_neutral moneyInReduceEffect.simps(2) moneyInReduceResult.simps(1) moneyInReduceResult.simps(2) moneyInReduceStepResult.simps(1) reduceContractStep_preserves_money reduceContractStep_preserves_validAndPositive_state)
 
 lemma reductionLoop_preserves_money_Payment_not_ReduceNoWarning :
@@ -451,14 +451,14 @@ lemma reductionLoop_preserves_money_Payment_not_ReduceNoWarning :
       moneyInState reSta +
       moneyInPayments (case ReduceWithPayment x2 of ReduceNoPayment \<Rightarrow> payments | ReduceWithPayment payment \<Rightarrow> payment # payments) =
       moneyInReduceResult (case ReduceWithPayment x2 of ReduceNoPayment \<Rightarrow> payments | ReduceWithPayment payment \<Rightarrow> payment # payments) reSta
-       (reductionLoop env reSta reCont (if reWa = ReduceNoWarning then warnings else reWa # warnings)
+       (reductionLoop reduced env reSta reCont (if reWa = ReduceNoWarning then warnings else reWa # warnings)
          (case ReduceWithPayment x2 of ReduceNoPayment \<Rightarrow> payments | ReduceWithPayment payment \<Rightarrow> payment # payments))) \<Longrightarrow>
    validAndPositive_state state \<Longrightarrow>
    reduceContractStep env state contract = Reduced reWa (ReduceWithPayment x2) reSta reCont \<Longrightarrow>
    reEf = ReduceWithPayment x2 \<Longrightarrow>
    reWa \<noteq> ReduceNoWarning \<Longrightarrow>
    moneyInState state + moneyInPayments payments =
-   moneyInReduceResult payments state (reductionLoop env reSta reCont (reWa # warnings) (x2 # payments))"
+   moneyInReduceResult payments state (reductionLoop reduced env reSta reCont (reWa # warnings) (x2 # payments))"
   by (smt ReduceEffect.simps(5) ReduceResult.exhaust moneyInPayments.simps(1) moneyInReduceEffect.simps(1) moneyInReduceResult.simps(1) moneyInReduceResult.simps(2) moneyInReduceStepResult.simps(1) reduceContractStep_preserves_money reduceContractStep_preserves_validAndPositive_state)
 
 lemma reductionLoop_preserves_money_Payment :
@@ -468,21 +468,21 @@ lemma reductionLoop_preserves_money_Payment :
               validAndPositive_state reSta \<Longrightarrow>
               moneyInState reSta +
               moneyInPayments xa =
-              moneyInReduceResult xa reSta (reductionLoop env reSta reCont warnings xa)) \<Longrightarrow>
+              moneyInReduceResult xa reSta (reductionLoop reduced env reSta reCont warnings xa)) \<Longrightarrow>
           validAndPositive_state state \<Longrightarrow>
           reduceContractStep env state contract = Reduced ReduceNoWarning (ReduceWithPayment x2) reSta reCont \<Longrightarrow>
           reEf = ReduceWithPayment x2 \<Longrightarrow>
           reWa = ReduceNoWarning \<Longrightarrow>
           moneyInState state + moneyInPayments payments =
-          moneyInReduceResult payments state (reductionLoop env reSta reCont warnings (x2 # payments))"
+          moneyInReduceResult payments state (reductionLoop reduced env reSta reCont warnings (x2 # payments))"
   by (smt ReduceEffect.simps(5) ReduceResult.exhaust moneyInPayments.simps(1) moneyInReduceEffect.simps(1) moneyInReduceResult.simps(1) moneyInReduceResult.simps(2) moneyInReduceStepResult.simps(1) reduceContractStep_preserves_money reduceContractStep_preserves_validAndPositive_state)
 
 lemma reductionLoop_preserves_money :
   "validAndPositive_state state \<Longrightarrow>
-   moneyInState state + moneyInPayments pa = moneyInReduceResult pa state (reductionLoop env state cont wa pa)"
-  apply (induction env state cont wa pa rule:reductionLoop.induct)
-  subgoal for env state contract warnings payments
-    apply (simp only:reductionLoop.simps[of env state contract warnings payments])
+   moneyInState state + moneyInPayments pa = moneyInReduceResult pa state (reductionLoop reduced env state cont wa pa)"
+  apply (induction reduced env state cont wa pa rule:reductionLoop.induct)
+  subgoal for reduced env state contract warnings payments
+    apply (simp only:reductionLoop.simps[of reduced env state contract warnings payments])
     apply (cases "reduceContractStep env state contract")
     subgoal for reWa reEf reSta reCont
       apply (cases reEf)
@@ -524,12 +524,12 @@ lemma moneyInPayments_distrib : "moneyInPayments (a @ b) = moneyInPayments a + m
 lemma applyAllLoop_preserves_money :
   "validAndPositive_state state \<Longrightarrow>
    moneyInState state + moneyInInputs inp + moneyInPayments pa
-    = moneyInApplyAllResult state inp pa (applyAllLoop env state cont inp wa pa)"
-  apply (induction env state cont inp wa pa rule:applyAllLoop.induct)
-  subgoal for env state contract inputs warnings payments
-    apply (simp only:applyAllLoop.simps[of env state contract inputs warnings payments])
+    = moneyInApplyAllResult state inp pa (applyAllLoop reduced env state cont inp wa pa)"
+  apply (induction reduced env state cont inp wa pa rule:applyAllLoop.induct)
+  subgoal for reduced env state contract inputs warnings payments
+    apply (simp only:applyAllLoop.simps[of reduced env state contract inputs warnings payments])
     apply (cases "reduceContractUntilQuiescent env state contract")
-    subgoal for redWa redPa redSta redCont
+    subgoal for redReduced redWa redPa redSta redCont
       apply (simp only:ReduceResult.simps)
       apply (cases "inputs")
       apply (simp only:list.simps)
@@ -540,7 +540,7 @@ lemma applyAllLoop_preserves_money :
         apply (cases "applyInput env redSta head redCont")
         apply (simp only:ApplyResult.simps moneyInApplyAllResult.simps)
         subgoal for appWarn appState appCont
-          apply (cases "(applyAllLoop env appState appCont tail (warnings @ convertReduceWarnings redWa @ convertApplyWarning appWarn) (payments @ redPa))")
+          apply (cases "(applyAllLoop True env appState appCont tail (warnings @ convertReduceWarnings redWa @ convertApplyWarning appWarn) (payments @ redPa))")
           apply (smt applyInput_preserves_money applyInput_preserves_preserves_validAndPositive_state moneyInApplyAllResult.simps(1) moneyInApplyResult.simps(1) moneyInInputs.simps(1) moneyInPayments_distrib moneyInReduceResult.simps(1) reduceContractUntilQuiescent_preserves_money reduceContractUntilQuiescent_preserves_validAndPositive_state)
           by simp_all
         by simp
@@ -569,9 +569,9 @@ lemma computeTransaction_preserves_money :
   subgoal for env fixSta
     apply (simp only:IntervalResult.simps Let_def)
     apply (cases "applyAllInputs env fixSta contract (inputs tra)")
-    subgoal for newWarn newPay newState newCont
+    subgoal for newReduced newWarn newPay newState newCont
       apply (simp only:ApplyAllResult.simps)
-      apply (cases "contract = newCont \<and> (contract \<noteq> Close \<or> accounts state = [])")
+      apply (cases "\<not> newReduced \<and> (contract \<noteq> Close \<or> accounts state = [])")
       apply (simp add:refl)
       apply (simp only:bool.case if_False)
       by (metis TransactionOutputRecord.select_convs(2) TransactionOutputRecord.select_convs(3) applyAllInputs_preserves_money fixInterval_preserves_money fixInterval_preserves_preserves_validAndPositive_state moneyInApplyAllResult.simps(1) moneyInTransactionOutput.simps(1))
