isabelle/SingleInputTransactions.thy
@@ -21,46 +21,46 @@ fun traceListToSingleInput :: "Transaction list \<Rightarrow> Transaction list" 
                               , inputs = inps \<rparr> rest) = inputsToTransactions si inps @ (traceListToSingleInput rest)"
 
 lemma reductionLoopIdempotent :
-  "reductionLoop env state contract wa pa = ContractQuiescent nwa npa nsta ncont \<Longrightarrow>
-   reductionLoop env nsta ncont [] [] = ContractQuiescent [] [] nsta ncont"  
-  apply (induction env state contract wa pa rule:reductionLoop.induct)
-  subgoal for env state contract warnings payments
+  "reductionLoop reducedBefore env state contract wa pa = ContractQuiescent reducedAfter nwa npa nsta ncont \<Longrightarrow>
+   reductionLoop reducedBefore2 env nsta ncont [] [] = ContractQuiescent reducedBefore2 [] [] nsta ncont"
+  apply (induction reducedBefore env state contract wa pa rule:reductionLoop.induct)
+  subgoal for reducedBefore env state contract warnings payments
     apply (cases "reduceContractStep env state contract")
     apply (cases "reduceContractStep env nsta ncont")
     apply (simp add:Let_def)
-    apply simp
-    apply simp
-    apply metis
+       apply simp
+       apply simp
+      apply metis
     apply simp
     by simp
   done
 
 lemma reduceContractUntilQuiescentIdempotent :           
-  "reduceContractUntilQuiescent env state contract = ContractQuiescent wa pa nsta ncont \<Longrightarrow>
-   reduceContractUntilQuiescent env nsta ncont = ContractQuiescent [] [] nsta ncont"
+  "reduceContractUntilQuiescent env state contract = ContractQuiescent reducedAfter wa pa nsta ncont \<Longrightarrow>
+   reduceContractUntilQuiescent env nsta ncont = ContractQuiescent False [] [] nsta ncont"
   apply (simp only:reduceContractUntilQuiescent.simps)
-  using reductionLoopIdempotent by blast  
+  using reductionLoopIdempotent by blast 
 
 lemma applyAllLoopEmptyIdempotent :
-  "applyAllLoop env sta cont [] a b = ApplyAllSuccess wa pa nsta ncont \<Longrightarrow>
-   applyAllLoop env nsta ncont [] c d = ApplyAllSuccess c d nsta ncont"
-  apply (simp only:applyAllLoop.simps[of env sta cont])
+  "applyAllLoop reducedBefore env sta cont [] a b = ApplyAllSuccess reducedAfter wa pa nsta ncont \<Longrightarrow>
+   applyAllLoop reducedBefore2 env nsta ncont [] c d = ApplyAllSuccess reducedBefore2 c d nsta ncont"
+  apply (simp only:applyAllLoop.simps[of reducedBefore env sta cont])
   apply (cases "reduceContractUntilQuiescent env sta cont")
   using reduceContractUntilQuiescentIdempotent apply auto[1]
   by simp
 
 lemma applyAllLoopJustAppendsWarningsAndEffects :
-  "applyAllLoop env st c list (wa @ wt) (ef @ et) = ApplyAllSuccess (wa @ nwa) (ef @ nef) fsta fcont \<Longrightarrow>
-   applyAllLoop env st c list (wa2 @ wt) (ef2 @ et) = ApplyAllSuccess (wa2 @ nwa) (ef2 @ nef) fsta fcont"
-  apply (induction list arbitrary: env st c wa wt ef et wa2 ef2 nwa nef)
-  subgoal for env st c wa wt ef et wa2 ef2 nwa nef
-    apply (simp only:applyAllLoop.simps[of env st c])
+  "applyAllLoop reducedBefore env st c list (wa @ wt) (ef @ et) = ApplyAllSuccess reducedAfter (wa @ nwa) (ef @ nef) fsta fcont \<Longrightarrow>
+   applyAllLoop reducedBefore env st c list (wa2 @ wt) (ef2 @ et) = ApplyAllSuccess reducedAfter (wa2 @ nwa) (ef2 @ nef) fsta fcont"
+  apply (induction list arbitrary: reducedBefore env st c wa wt ef et wa2 ef2 nwa nef)
+  subgoal for reducedBefore env st c wa wt ef et wa2 ef2 nwa nef
+    apply (simp only:applyAllLoop.simps[of reducedBefore env st c])
     apply (cases "reduceContractUntilQuiescent env st c")
     by simp_all
-  subgoal for head tail env st c wa wt ef et wa2 ef2 nwa nef
-    apply (simp only:applyAllLoop.simps[of env st c "(head # tail)"])
+  subgoal for head tail reducedBefore env st c wa wt ef et wa2 ef2 nwa nef
+    apply (simp only:applyAllLoop.simps[of reducedBefore env st c "(head # tail)"])
     apply (cases "reduceContractUntilQuiescent env st c")
-    subgoal for tempWa tempEf tempState tempContract
+    subgoal for tempReducedAfter tempWa tempEf tempState tempContract
       apply (simp only:ReduceResult.case)
       apply (subst list.case(2)[of _ _ head tail])
       apply (subst (asm) list.case(2)[of _ _ head tail])
@@ -70,105 +70,165 @@ lemma applyAllLoopJustAppendsWarningsAndEffects :
     by simp
   done
 
+lemma applyAllLoop_preserves_reduced : "applyAllLoop True env state cont list warns pays = ApplyAllSuccess reduced fwarn fpays fstate fcont \<Longrightarrow> reduced"
+  apply (induction "True" env state cont list warns pays arbitrary:reduced fwarn fpays fstate fcont rule:applyAllLoop.induct)
+  subgoal for env state contract inputs warnings payments reduced fwarn fpays fstate fcont
+    apply (simp only:applyAllLoop.simps[of True env state])
+    apply (auto split:ReduceResult.splits list.splits ApplyResult.splits simp del:reduceContractUntilQuiescent.simps applyAllLoop.simps applyInput.simps simp add:Let_def refl)
+    by blast
+  done
+
+lemma applyAllLoop_noNil_reduces : "applyAllLoop False env sta cont (h#t) wa ef = ApplyAllSuccess reduced nwa npa nsta ncont \<Longrightarrow> reduced"
+  apply (simp only:applyAllLoop.simps[of False env])
+  apply (auto split:ReduceResult.splits ApplyResult.splits simp del:reduceContractUntilQuiescent.simps applyInput.simps applyAllLoop.simps)
+  using applyAllLoop_preserves_reduced by blast
+
+lemma sthOrInequality : "(reducedBefore \<or> a # list \<noteq> []) = True"
+  by simp
+
 lemma applyLoopIdempotent_base_case :
-  "applyAllLoop env sta cont [] twa tef = ApplyAllSuccess wa pa nsta ncont \<Longrightarrow>
-   applyAllLoop env sta cont t twa tef = ApplyAllSuccess (wa @ nwa) (pa @ npa) fsta fcont \<Longrightarrow>
-   applyAllLoop env nsta ncont t [] [] = ApplyAllSuccess nwa npa fsta fcont"
-  apply (simp only:applyAllLoop.simps[of env sta cont])
+  "applyAllLoop reducedBefore env sta cont [] twa tef = ApplyAllSuccess reducedAfter wa pa nsta ncont \<Longrightarrow>
+   applyAllLoop reducedBefore env sta cont t twa tef = ApplyAllSuccess reducedAfter2 (wa @ nwa) (pa @ npa) fsta fcont \<Longrightarrow>
+   applyAllLoop reducedBefore2 env nsta ncont t [] [] = ApplyAllSuccess (reducedBefore2 \<or> (t \<noteq> [])) nwa npa fsta fcont"
+  apply (simp only:applyAllLoop.simps[of reducedBefore env sta cont])
   apply (cases "reduceContractUntilQuiescent env sta cont")
   apply (simp only:ReduceResult.case list.case)
-  apply (simp only:applyAllLoop.simps[of env nsta ncont])
+  apply (simp only:applyAllLoop.simps[of reducedBefore2 env nsta ncont])
   apply (cases "reduceContractUntilQuiescent env nsta ncont")
   apply (simp only:ReduceResult.case list.case)
   apply (cases t)
   apply (simp only:list.case)
   using reduceContractUntilQuiescentIdempotent apply auto[1]
   apply (simp only:list.case)
-  subgoal for x11 x12 x13 x14 x11a x12a x13a x14a a list
-    apply (cases "applyInput env x13a a x14a")
-    apply (cases "applyInput env x13 a x14")
-    apply (simp only:ApplyResult.case)
-    apply (smt ApplyAllResult.inject ApplyResult.inject ReduceResult.inject append.right_neutral append_assoc applyAllLoopJustAppendsWarningsAndEffects convertReduceWarnings.simps(1) reduceContractUntilQuiescentIdempotent self_append_conv2)
+  subgoal for x11 x12 x13 x14 x15 x11a x12a x13a x14a x15a a list
+    apply (cases "applyInput env x14a a x15a")
+    apply (cases "applyInput env x14 a x15")
+      apply (simp only:ApplyResult.case sthOrInequality)
+    apply (smt ApplyAllResult.inject ApplyResult.inject ReduceResult.inject append.right_neutral append_assoc applyAllLoopJustAppendsWarningsAndEffects applyAllLoop_preserves_reduced convertReduceWarnings.simps(1) reduceContractUntilQuiescentIdempotent self_append_conv2)
     using reduceContractUntilQuiescentIdempotent apply auto[1]
     using reduceContractUntilQuiescentIdempotent by auto
   using reduceContractUntilQuiescentIdempotent apply auto[1]
   by auto
 
 lemma applyLoopIdempotent :
-  "applyAllLoop env sta cont [h] [] [] = ApplyAllSuccess wa pa nsta ncont \<Longrightarrow>
-   applyAllLoop env sta cont (h # t) [] [] = ApplyAllSuccess (wa @ nwa) (pa @ npa) fsta fcont \<Longrightarrow>
-   applyAllLoop env nsta ncont t [] [] = ApplyAllSuccess nwa npa fsta fcont"
-  apply (simp only:applyAllLoop.simps[of env sta cont])
+  "applyAllLoop reducedBefore env sta cont [h] [] [] = ApplyAllSuccess reducedAfter wa pa nsta ncont \<Longrightarrow>
+   applyAllLoop reducedBefore env sta cont (h # t) [] [] = ApplyAllSuccess reducedAfter2 (wa @ nwa) (pa @ npa) fsta fcont \<Longrightarrow>
+   applyAllLoop reducedBefore env nsta ncont t [] [] = ApplyAllSuccess (reducedBefore \<or> (t \<noteq> [])) nwa npa fsta fcont"
+  apply (simp only:applyAllLoop.simps[of reducedBefore env sta cont])
   apply (cases "reduceContractUntilQuiescent env sta cont")
   apply (simp only:ReduceResult.case Let_def list.case)
-  subgoal for x11 x12 x13 x14
-    apply (cases "applyInput env x13 h x14")
+  subgoal for x11 x12 x13 x14 x15
+    apply (cases "applyInput env x14 h x15")
     subgoal for x11a x12a x13a
+      apply (simp only:applyInput.simps refl ApplyResult.case)
       using applyLoopIdempotent_base_case by auto
     by simp
   by simp
  
  lemma applyLoopIdempotent_base_case2 :
-   "applyAllLoop env sta cont [] twa tef = ApplyAllSuccess wa pa nsta ncont \<Longrightarrow>
-   applyAllLoop env nsta ncont t [] [] = ApplyAllSuccess nwa npa fsta fcont \<Longrightarrow>
-   applyAllLoop env sta cont t twa tef = ApplyAllSuccess (wa @ nwa) (pa @ npa) fsta fcont"
-   apply (simp only:applyAllLoop.simps[of env sta cont])
+   "applyAllLoop reducedBefore env sta cont [] twa tef = ApplyAllSuccess reducedAfter wa pa nsta ncont \<Longrightarrow>
+   applyAllLoop reducedAfter env nsta ncont t [] [] = ApplyAllSuccess reducedAfter2 nwa npa fsta fcont \<Longrightarrow>
+   applyAllLoop reducedBefore env sta cont t twa tef = ApplyAllSuccess reducedAfter2 (wa @ nwa) (pa @ npa) fsta fcont"
+   apply (simp only:applyAllLoop.simps[of reducedBefore env sta cont])
    apply (cases "reduceContractUntilQuiescent env sta cont")
    apply (simp only:ReduceResult.case list.case)
-   apply (simp only:applyAllLoop.simps[of env nsta ncont])
+   apply (simp only:applyAllLoop.simps[of reducedAfter env nsta ncont])
    apply (cases "reduceContractUntilQuiescent env nsta ncont")
    apply (simp only:ReduceResult.case list.case)
    apply (cases t)
-   apply (simp only:list.case)
    using reduceContractUntilQuiescentIdempotent apply auto[1]
-   apply (simp only:list.case)
-   subgoal for x11 x12 x13 x14 x11a x12a x13a x14a a list
-     apply (cases "applyInput env x13a a x14a")
-     apply (cases "applyInput env x13 a x14")
-     apply (simp only:ApplyResult.case)
-     apply (smt ApplyAllResult.inject ApplyResult.inject ReduceResult.inject append.right_neutral append_assoc applyAllLoopJustAppendsWarningsAndEffects convertReduceWarnings.simps(1) reduceContractUntilQuiescentIdempotent self_append_conv2)
-     using reduceContractUntilQuiescentIdempotent apply auto[1]
+   apply (simp only:list.case ApplyResult.case)
+   subgoal for x11 x12 x13 x14 x15 x11a x12a x13a x14a x15a a list
+     apply (cases "applyInput env x14a a x15a")
+     apply (cases "applyInput env x14 a x15")
+       apply (simp only:ApplyResult.case)
+     subgoal for x11b x12b x13b x11aa x12aa x13aa
+         proof -
+           assume a1: "ApplyAllSuccess (reducedBefore \<or> x11) (twa @ convertReduceWarnings x12) (tef @ x13) x14 x15 = ApplyAllSuccess reducedAfter wa pa nsta ncont"
+           assume a2: "reduceContractUntilQuiescent env sta cont = ContractQuiescent x11 x12 x13 x14 x15"
+           assume a3: "reduceContractUntilQuiescent env nsta ncont = ContractQuiescent x11a x12a x13a x14a x15a"
+           assume a4: "applyInput env x14a a x15a = Applied x11b x12b x13b"
+      assume a5: "applyInput env x14 a x15 = Applied x11aa x12aa x13aa"
+        assume a6: "applyAllLoop True env x12b x13b list ([] @ convertReduceWarnings x12a @ convertApplyWarning x11b) ([] @ x13a) = ApplyAllSuccess reducedAfter2 nwa npa fsta fcont"
+        have f7: "(\<not> reducedBefore \<and> \<not> x11) \<noteq> reducedAfter \<and> twa @ convertReduceWarnings x12 = wa \<and> tef @ x13 = pa \<and> x14 = nsta \<and> x15 = ncont"
+          using a1 by blast
+        have "reduceContractUntilQuiescent env x14 x15 = ContractQuiescent False [] [] x14 x15"
+          using a2 by (meson reduceContractUntilQuiescentIdempotent)
+        then have f8: "\<not> x11a \<and> [] = x12a \<and> [] = [] @ x13a \<and> nsta = x14a \<and> ncont = x15a"
+          using f7 a3 by simp
+        then have f9: "[] = convertReduceWarnings x12a"
+          using convertReduceWarnings.simps(1) by presburger
+        have f10: "wa @ [] @ convertReduceWarnings x12a @ convertApplyWarning x11b = twa @ convertReduceWarnings x12 @ convertApplyWarning x11aa"
+          using f8 f7 a5 a4 by simp
+        have f11: "applyAllLoop True env x12aa x13aa list (convertReduceWarnings x12a @ [] @ convertReduceWarnings x12a @ convertApplyWarning x11b) (([] @ x13a) @ [] @ x13a) = ApplyAllSuccess reducedAfter2 nwa npa fsta fcont"
+          using f8 f7 a6 a5 a4 by auto
+        have "convertReduceWarnings x12a @ [] @ nwa = nwa"
+      using f9 by auto
+        then show ?thesis
+          using f11 f10 f8 f7 by (metis (no_types) append.right_neutral applyAllLoopJustAppendsWarningsAndEffects self_append_conv2)
+      qed
+      using reduceContractUntilQuiescentIdempotent apply auto[1]
+      by simp
+     apply simp
     by simp
-   apply simp
-  by simp
- 
- lemma applyLoopIdempotent2 :
-   "applyAllLoop env sta cont [h] [] [] = ApplyAllSuccess wa pa nsta ncont \<Longrightarrow>
-   applyAllLoop env nsta ncont t [] [] = ApplyAllSuccess nwa npa fsta fcont \<Longrightarrow>
-   applyAllLoop env sta cont (h # t) [] [] = ApplyAllSuccess (wa @ nwa) (pa @ npa) fsta fcont"
-   apply (simp only:applyAllLoop.simps[of env sta cont])
+
+lemma applyLoopIdempotent2 :
+   "applyAllLoop reducedBefore env sta cont [h] [] [] = ApplyAllSuccess reducedAfter wa pa nsta ncont \<Longrightarrow>
+   applyAllLoop reducedAfter env nsta ncont t [] [] = ApplyAllSuccess reducedAfter2 nwa npa fsta fcont \<Longrightarrow>
+   applyAllLoop reducedBefore env sta cont (h # t) [] [] = ApplyAllSuccess reducedAfter2 (wa @ nwa) (pa @ npa) fsta fcont"
+   apply (simp only:applyAllLoop.simps[of reducedBefore env sta cont])
    apply (cases "reduceContractUntilQuiescent env sta cont")
    apply (simp only:ReduceResult.case Let_def list.case)
-   subgoal for x11 x12 x13 x14
-     apply (cases "applyInput env x13 h x14")
-     subgoal for x11a x12a x13a
-       using applyLoopIdempotent_base_case2 by auto
-     by simp
+   subgoal for x11 x12 x13 x14 x15
+     apply (cases "applyInput env x14 h x15")
+     subgoal for x12a x13a x14a
+       apply (simp only:ApplyResult.case)
+       using applyLoopIdempotent_base_case2 by blast
+     using applyLoopIdempotent_base_case2 by auto
    by simp
 
-
 lemma applyAllIterative :
-  "applyAllInputs env sta cont [h] = ApplyAllSuccess wa pa nsta ncont \<Longrightarrow>
-   applyAllInputs env sta cont (h#t) = ApplyAllSuccess (wa @ nwa) (pa @ npa) fsta fcont \<Longrightarrow>
-   applyAllInputs env nsta ncont t = ApplyAllSuccess nwa npa fsta fcont"
+  "applyAllInputs env sta cont [h] = ApplyAllSuccess reducedAfter wa pa nsta ncont \<Longrightarrow>
+   applyAllInputs env sta cont (h#t) = ApplyAllSuccess reducedAfter2 (wa @ nwa) (pa @ npa) fsta fcont \<Longrightarrow>
+   applyAllInputs env nsta ncont t = ApplyAllSuccess (t \<noteq> []) nwa npa fsta fcont"
   apply (simp only:applyAllInputs.simps)
-  using applyLoopIdempotent by blast
+  by (smt applyLoopIdempotent)
+
+lemma applyAllIterative2_aux :
+  "applyAllInputs env sta cont [h] = ApplyAllSuccess True wa pa nsta ncont \<Longrightarrow>
+  applyAllInputs env nsta ncont t = ApplyAllSuccess reduceAfter2 nwa npa fsta fcont \<Longrightarrow>
+  applyAllInputs env sta cont (h#t) = ApplyAllSuccess True (wa @ nwa) (pa @ npa) fsta fcont"
+  apply (simp only:applyAllInputs.simps)
+  proof -
+    assume a1: "applyAllLoop False env sta cont [h] [] [] = ApplyAllSuccess True wa pa nsta ncont"
+    assume a2: "applyAllLoop False env nsta ncont t [] [] = ApplyAllSuccess reduceAfter2 nwa npa fsta fcont"
+    have f3: "\<forall>b e s c i ba ts ps sa ca is bb tsa psa sb cb. applyAllLoop b e s c [i] [] [] \<noteq> ApplyAllSuccess ba ts ps sa ca \<or> applyAllLoop b e s c (i # is) [] [] \<noteq> ApplyAllSuccess bb (ts @ tsa) (ps @ psa) sb cb \<or> applyAllLoop b e sa ca is [] [] = ApplyAllSuccess (b \<or> is \<noteq> []) tsa psa sb cb"
+      by (meson applyLoopIdempotent)
+    have "applyAllLoop False env sta cont [h] [] [] = ApplyAllSuccess True (wa @ []) (pa @ []) nsta ncont"
+      using a1 by simp
+    then have "applyAllLoop False env nsta ncont [] [] [] = ApplyAllSuccess False [] [] nsta ncont"
+      using f3 a1 by presburger
+    then show "applyAllLoop False env sta cont (h # t) [] [] = ApplyAllSuccess True (wa @ nwa) (pa @ npa) fsta fcont"
+      using a2 a1 applyLoopIdempotent2 applyLoopIdempotent_base_case by auto
+  qed
 
 lemma applyAllIterative2 :
-  "applyAllInputs env sta cont [h] = ApplyAllSuccess wa pa nsta ncont \<Longrightarrow>
-  applyAllInputs env nsta ncont t = ApplyAllSuccess nwa npa fsta fcont \<Longrightarrow>
-  applyAllInputs env sta cont (h#t) = ApplyAllSuccess (wa @ nwa) (pa @ npa) fsta fcont"
-  apply (simp only:applyAllInputs.simps)
-  using applyLoopIdempotent2 by blast
+  "applyAllInputs env sta cont [h] = ApplyAllSuccess reduceAfter1 wa pa nsta ncont \<Longrightarrow>
+  applyAllInputs env nsta ncont t = ApplyAllSuccess reduceAfter2 nwa npa fsta fcont \<Longrightarrow>
+  applyAllInputs env sta cont (h#t) = ApplyAllSuccess True (wa @ nwa) (pa @ npa) fsta fcont"
+  apply (rule mp[of "reduceAfter1 = True"])
+  using applyAllIterative2_aux apply blast
+  apply (simp only:applyAllInputs.simps[of env sta cont "[h]"])
+  using applyAllLoop_noNil_reduces by blast
 
 lemma applyAllInputsPrefix1:
-  "applyAllLoop env sta cont l iwa ipa = ApplyAllSuccess fwa fpa nsta ncont \<Longrightarrow>
+  "applyAllLoop reduceBefore env sta cont l iwa ipa = ApplyAllSuccess reduceAfter fwa fpa nsta ncont \<Longrightarrow>
    \<exists>nwa. fwa = iwa @ nwa"
-  apply (induction env sta cont l iwa ipa arbitrary:fwa fpa nsta ncont rule:applyAllLoop.induct)
-  subgoal for env state contract inputs warnings payments fwa fpa nsta ncont
-    apply (simp only:applyAllLoop.simps[of env state contract inputs warnings payments])
+  apply (induction reduceBefore env sta cont l iwa ipa arbitrary:fwa fpa nsta ncont rule:applyAllLoop.induct)
+  subgoal for reduceBefore env state contract inputs warnings payments fwa fpa nsta ncont
+    apply (simp only:applyAllLoop.simps[of reduceBefore env state contract inputs warnings payments])
     apply (cases "reduceContractUntilQuiescent env state contract")
-    subgoal for reduceWarns reducePays reduceState reduceCont
+    subgoal for reduceReduced reduceWarns reducePays reduceState reduceCont
       apply (simp only:ReduceResult.case)
       apply (cases inputs)
       apply (simp only:list.case)
@@ -177,21 +237,21 @@ lemma applyAllInputsPrefix1:
         apply (simp only:list.case)
         apply (cases "applyInput env reduceState h reduceCont")
         subgoal for applyWarn applyState applyCont
-        apply (simp only:ApplyResult.case)
-          using append.assoc by blast
+          apply (simp only:ApplyResult.case)
+          by fastforce
         by simp
       done
     by simp
   done
 
 lemma applyAllInputsPrefix2:
-  "applyAllLoop env sta cont l iwa ipa = ApplyAllSuccess fwa fpa nsta ncont \<Longrightarrow>
+  "applyAllLoop reducedBefore env sta cont l iwa ipa = ApplyAllSuccess reducedAfter fwa fpa nsta ncont \<Longrightarrow>
    \<exists>npa. fpa = ipa @ npa"
-  apply (induction env sta cont l iwa ipa arbitrary:fwa fpa nsta ncont rule:applyAllLoop.induct)
-  subgoal for env state contract inputs warnings payments fwa fpa nsta ncont
-    apply (simp only:applyAllLoop.simps[of env state contract inputs warnings payments])
+  apply (induction reducedBefore env sta cont l iwa ipa arbitrary:reducedAfter fwa fpa nsta ncont rule:applyAllLoop.induct)
+  subgoal for reducedBefore env state contract inputs warnings payments reducedAfter fwa fpa nsta ncont
+    apply (simp only:applyAllLoop.simps[of reducedBefore env state contract inputs warnings payments])
     apply (cases "reduceContractUntilQuiescent env state contract")
-    subgoal for reduceWarns reducePays reduceState reduceCont
+    subgoal for reduceReduced reduceWarns reducePays reduceState reduceCont
       apply (simp only:ReduceResult.case)
       apply (cases inputs)
       apply (simp only:list.case)
@@ -200,8 +260,8 @@ lemma applyAllInputsPrefix2:
         apply (simp only:list.case)
         apply (cases "applyInput env reduceState h reduceCont")
         subgoal for applyWarn applyState applyCont
-        apply (simp only:ApplyResult.case)
-          using append.assoc by blast
+         apply (simp only:ApplyResult.case)
+          by force
         by simp
       done
     by simp
@@ -210,11 +270,11 @@ lemma applyAllInputsPrefix2:
 lemma beforeApplyAllLoopIsUseless:
   "iwa @ convertReduceWarnings x11 = wa \<Longrightarrow>
    ipa @ x12 = pa \<Longrightarrow>
-   applyAllLoop env applyState applyCont t iwa ipa = ApplyAllSuccess fwa fpa fsta fcont \<Longrightarrow>
-   reduceContractUntilQuiescent env applyState applyCont = ContractQuiescent x11 x12 nsta ncont \<Longrightarrow>
-   ApplyAllSuccess fwa fpa fsta fcont = applyAllLoop env nsta ncont t wa pa"
-  apply (simp only:applyAllLoop.simps[of env applyState])
-  apply (simp only:applyAllLoop.simps[of env nsta])
+   applyAllLoop reducedBefore2 env applyState applyCont t iwa ipa = ApplyAllSuccess reducedAfter2 fwa fpa fsta fcont \<Longrightarrow>
+   reduceContractUntilQuiescent env applyState applyCont = ContractQuiescent reducedAfter x11 x12 nsta ncont \<Longrightarrow>
+   ApplyAllSuccess reducedAfter2 fwa fpa fsta fcont = applyAllLoop reducedAfter2 env nsta ncont t wa pa"
+  apply (simp only:applyAllLoop.simps[of reducedBefore2 env applyState])
+  apply (simp only:applyAllLoop.simps[of reducedAfter2 env nsta])
   apply (cases "reduceContractUntilQuiescent env nsta ncont")
   subgoal for x11a x12a x13 x14
   apply (simp only:ReduceResult.case)
@@ -231,22 +291,22 @@ lemma beforeApplyAllLoopIsUseless:
   using reduceContractUntilQuiescentIdempotent by auto
 
 lemma applyAllInputsPrefix_aux:
-  "applyAllLoop env sta cont [h] [] [] = ApplyAllSuccess wa pa nsta ncont \<Longrightarrow>
-   applyAllLoop env sta cont (h # t) [] [] = ApplyAllSuccess fwa fpa fsta fcont \<Longrightarrow>
-   (\<exists> twa x11 x12 applyState applyCont reducePays reduceState reduceCont.
-    twa @ convertReduceWarnings x11 = wa \<and>
-    reducePays @ x12 = pa \<and>
-    applyAllLoop env applyState applyCont t twa reducePays = ApplyAllSuccess fwa fpa fsta fcont \<and>
-    reduceContractUntilQuiescent env applyState applyCont = ContractQuiescent x11 x12 nsta ncont)"
-    apply (subst (asm) applyAllLoop.simps[of env sta cont "[h]"])
+  "applyAllLoop reducedBefore env sta cont [h] [] [] = ApplyAllSuccess reducedAfter wa pa nsta ncont \<Longrightarrow>
+   applyAllLoop reducedBefore2 env sta cont (h # t) [] [] = ApplyAllSuccess reducedAfter2 fwa fpa fsta fcont \<Longrightarrow>
+   (\<exists> applyReducedBefore twa x11 x12 x13 applyState applyCont reducePays reduceState reduceCont.
+    twa @ convertReduceWarnings x12 = wa \<and>
+    reducePays @ x13 = pa \<and>
+    applyAllLoop applyReducedBefore env applyState applyCont t twa reducePays = ApplyAllSuccess reducedAfter2 fwa fpa fsta fcont \<and>
+    reduceContractUntilQuiescent env applyState applyCont = ContractQuiescent x11 x12 x13 nsta ncont)"
+    apply (subst (asm) applyAllLoop.simps[of reducedBefore env sta cont "[h]"])
     apply (cases "reduceContractUntilQuiescent env sta cont")
-    subgoal for reduceWarns reducePays reduceState reduceCont
+    subgoal for reduceReduced reduceWarns reducePays reduceState reduceCont
       apply (simp only:ReduceResult.case)
       apply (simp only:list.case)
       apply (cases "applyInput env reduceState h reduceCont")
       subgoal for applyWarn applyState applyCont
         apply (simp only:ApplyResult.case)
-    apply (subst (asm) applyAllLoop.simps[of env sta cont "(h # t)"])
+    apply (subst (asm) applyAllLoop.simps[of reducedBefore2 env sta cont "(h # t)"])
     apply (cases "reduceContractUntilQuiescent env sta cont")
     subgoal for reduceWarns2 reducePays2 reduceState2 reduceCont2
       apply (simp only:ReduceResult.case)
@@ -254,7 +314,7 @@ lemma applyAllInputsPrefix_aux:
       apply (cases "applyInput env reduceState h reduceCont")
       subgoal for applyWarn2 applyState2 applyCont2
         apply (simp only:ApplyResult.case)
-        apply (subst (asm) applyAllLoop.simps[of env applyState applyCont "[]"])
+        apply (subst (asm) applyAllLoop.simps[of True env applyState applyCont "[]"])
         apply (cases "reduceContractUntilQuiescent env applyState applyCont")
         subgoal for x11 x12 x13 x14
           apply (simp only:ReduceResult.case list.case)
@@ -267,31 +327,31 @@ lemma applyAllInputsPrefix_aux:
   by simp
 
 lemma applyAllInputsPrefix1_aux2:
-  "applyAllLoop env sta cont [h] [] [] = ApplyAllSuccess wa pa nsta ncont \<Longrightarrow>
-   applyAllLoop env sta cont (h # t) [] [] = ApplyAllSuccess fwa fpa fsta fcont \<Longrightarrow>
+  "applyAllLoop reducedBefore env sta cont [h] [] [] = ApplyAllSuccess reducedAfter wa pa nsta ncont \<Longrightarrow>
+   applyAllLoop reducedBefore2 env sta cont (h # t) [] [] = ApplyAllSuccess reducedAfter2 fwa fpa fsta fcont \<Longrightarrow>
    \<exists>nwa. fwa = wa @ nwa"
-  apply (frule applyAllInputsPrefix_aux[of env sta cont h wa pa nsta ncont t fwa fpa fsta fcont])
+  apply (frule applyAllInputsPrefix_aux[of reducedBefore env sta cont h reducedAfter wa pa nsta ncont reducedBefore2 t reducedAfter2 fwa fpa fsta fcont])
   apply simp
   by (metis applyAllInputsPrefix1 beforeApplyAllLoopIsUseless)
 
 lemma applyAllPrefix1:
-  "applyAllInputs env sta cont [h] = ApplyAllSuccess wa pa nsta ncont \<Longrightarrow>
-   applyAllInputs env sta cont (h#t) = ApplyAllSuccess fwa fpa fsta fcont \<Longrightarrow>
+  "applyAllInputs env sta cont [h] = ApplyAllSuccess reducedAfter wa pa nsta ncont \<Longrightarrow>
+   applyAllInputs env sta cont (h#t) = ApplyAllSuccess reducedAfter2 fwa fpa fsta fcont \<Longrightarrow>
    (\<exists> nwa. fwa = wa @ nwa)"
   apply (simp only:applyAllInputs.simps)
   by (simp add: applyAllInputsPrefix1_aux2)
 
 lemma applyAllInputsPrefix2_aux2:
-  "applyAllLoop env sta cont [h] [] [] = ApplyAllSuccess wa pa nsta ncont \<Longrightarrow>
-   applyAllLoop env sta cont (h # t) [] [] = ApplyAllSuccess fwa fpa fsta fcont \<Longrightarrow>
+  "applyAllLoop reducedBefore env sta cont [h] [] [] = ApplyAllSuccess reducedAfter wa pa nsta ncont \<Longrightarrow>
+   applyAllLoop reducedBefore2 env sta cont (h # t) [] [] = ApplyAllSuccess reducedAfter2 fwa fpa fsta fcont \<Longrightarrow>
    \<exists>npa. fpa = pa @ npa"
-  apply (frule applyAllInputsPrefix_aux[of env sta cont h wa pa nsta ncont t fwa fpa fsta fcont])
+  apply (frule applyAllInputsPrefix_aux[of reducedBefore env sta cont h reducedAfter wa pa nsta ncont reducedBefore2 t reducedAfter2 fwa fpa fsta fcont])
   apply simp
   by (metis applyAllInputsPrefix2 beforeApplyAllLoopIsUseless)
 
 lemma applyAllPrefix2:
-  "applyAllInputs env sta cont [h] = ApplyAllSuccess wa pa nsta ncont \<Longrightarrow>
-   applyAllInputs env sta cont (h#t) = ApplyAllSuccess fwa fpa fsta fcont \<Longrightarrow>
+  "applyAllInputs env sta cont [h] = ApplyAllSuccess reduced wa pa nsta ncont \<Longrightarrow>
+   applyAllInputs env sta cont (h#t) = ApplyAllSuccess reduced2 fwa fpa fsta fcont \<Longrightarrow>
    (\<exists> npa. fpa = pa @ npa)"
   by (simp add: applyAllInputsPrefix2_aux2)
 
@@ -382,8 +442,8 @@ lemma reductionContractStep_preserves_minSlot :
   by (metis ReduceStepResult.distinct(1) ReduceStepResult.distinct(3) ReduceStepResult.inject)
 
 lemma reductionLoop_preserves_minSlot :
-  "reductionLoop env sta con wa pa = ContractQuiescent reduceWarns pays sta2 con2 \<Longrightarrow> minSlot sta = minSlot sta2"
-  apply (induction env sta con wa pa arbitrary:reduceWarns pays sta2 con2 rule:reductionLoop.induct)
+  "reductionLoop reducedBefore env sta con wa pa = ContractQuiescent reducedAfter reduceWarns pays sta2 con2 \<Longrightarrow> minSlot sta = minSlot sta2"
+  apply (induction reducedBefore env sta con wa pa arbitrary:reducedAfter reduceWarns pays sta2 con2 rule:reductionLoop.induct)
   subgoal for env state contract warnings payments reduceWarns pays sta2 con2
     apply (simp only:reductionLoop.simps[of env state contract warnings payments])
     apply (auto split:ReduceStepResult.splits simp del:reductionLoop.simps)
@@ -391,7 +451,7 @@ lemma reductionLoop_preserves_minSlot :
   done
 
 lemma reduceContractUntilQuiescent_preserves_minSlot :
-  "reduceContractUntilQuiescent env sta con = ContractQuiescent reduceWarns pays sta2 con2 \<Longrightarrow> minSlot sta = minSlot sta2"
+  "reduceContractUntilQuiescent env sta con = ContractQuiescent reducedAfter reduceWarns pays sta2 con2 \<Longrightarrow> minSlot sta = minSlot sta2"
   apply (simp only:reduceContractUntilQuiescent.simps)
   by (simp add: reductionLoop_preserves_minSlot)
 
@@ -416,20 +476,20 @@ lemma applyInput_preserves_minSlot :
   by (auto simp add:applyCases_preserves_minSlot)
 
 lemma applyAllLoop_preserves_minSlot :
-  "applyAllLoop env sta con inp wa pa = ApplyAllSuccess wa2 pa2 sta2 con2 \<Longrightarrow> minSlot sta = minSlot sta2"
-  apply (induction inp arbitrary:env sta con wa pa wa2 pa2 sta2 con2)
-  subgoal for env sta con wa pa wa2 pa2 sta2 con2
-    apply (simp only:applyAllLoop.simps[of env sta con "[]" wa pa])
+  "applyAllLoop reducedBefore env sta con inp wa pa = ApplyAllSuccess reducedAfter wa2 pa2 sta2 con2 \<Longrightarrow> minSlot sta = minSlot sta2"
+  apply (induction inp arbitrary:reducedBefore env sta con wa pa reducedAfter wa2 pa2 sta2 con2)
+  subgoal for reducedBefore env sta con wa pa reducedAfter wa2 pa2 sta2 con2
+    apply (simp only:applyAllLoop.simps[of reducedBefore env sta con "[]" wa pa])
     apply (cases "reduceContractUntilQuiescent env sta con")
     subgoal for reduceWarns pays curState cont
       apply (simp del:reduceContractUntilQuiescent.simps)
       using reduceContractUntilQuiescent_preserves_minSlot by blast
       apply (simp del:reduceContractUntilQuiescent.simps)
     done
-  subgoal for head tail env sta con wa pa wa2 pa2 sta2 con2
-      apply (simp only:applyAllLoop.simps[of env sta con "(head # tail)" wa pa])
+  subgoal for head tail reducedBefore env sta con wa pa reducedAfter wa2 pa2 sta2 con2
+      apply (simp only:applyAllLoop.simps[of reducedBefore env sta con "(head # tail)" wa pa])
       apply (cases "reduceContractUntilQuiescent env sta con")
-      subgoal for reduceWarns pays curState cont
+      subgoal for reducedAfter reduceWarns pays curState cont
         apply (cases "applyInput env curState head cont")
         subgoal for applyWarn newState newCont
           by (simp add: applyInput_preserves_minSlot reduceContractUntilQuiescent_preserves_minSlot)
@@ -438,19 +498,19 @@ lemma applyAllLoop_preserves_minSlot :
     done
 
 lemma applyAllInputs_preserves_minSlot :
-  "applyAllInputs env sta con inp = ApplyAllSuccess wa2 pa2 sta2 con2 \<Longrightarrow>
+  "applyAllInputs env sta con inp = ApplyAllSuccess reducedAfter wa2 pa2 sta2 con2 \<Longrightarrow>
    minSlot sta = minSlot sta2"
   apply (simp only:applyAllInputs.simps)
   using applyAllLoop_preserves_minSlot by blast
 
 lemma applyAllInputs_preserves_minSlot_rev :
-   "applyAllInputs env sta con inp = ApplyAllSuccess wa2 pa2 sta2 con2 \<Longrightarrow>
+   "applyAllInputs env sta con inp = ApplyAllSuccess reducedAfter wa2 pa2 sta2 con2 \<Longrightarrow>
     minSlot sta2 = minSlot sta"
   by (simp add: applyAllInputs_preserves_minSlot)
 
 lemma fixIntervalIdempotentThroughApplyAllInputs :
   "fixInterval inte sta1 = IntervalTrimmed env2 sta2 \<Longrightarrow>
-   applyAllInputs env2 sta2 con3 inp1 = ApplyAllSuccess wa4 pa4 sta4 con4 \<Longrightarrow>
+   applyAllInputs env2 sta2 con3 inp1 = ApplyAllSuccess reducedAfter wa4 pa4 sta4 con4 \<Longrightarrow>
    fixInterval inte sta4 = IntervalTrimmed env2 sta4"
   apply (cases env2)
   subgoal for slotInterval
@@ -466,9 +526,10 @@ lemma fixIntervalIdempotentThroughApplyAllInputs :
       done
     done
   done
+
 lemma fixIntervalIdempotentThroughApplyAllInputs2 :
   "fixInterval interv sta = IntervalTrimmed fIenv1 fIsta1 \<Longrightarrow>
-   applyAllInputs fIenv1 fIsta1 con [head] = ApplyAllSuccess iwa ipa ista con3 \<Longrightarrow>
+   applyAllInputs fIenv1 fIsta1 con [head] = ApplyAllSuccess reducedAfter iwa ipa ista con3 \<Longrightarrow>
    fixInterval interv ista = IntervalTrimmed fIenv1 ista"
   using fixIntervalIdempotentThroughApplyAllInputs by blast
 
@@ -513,11 +574,11 @@ lemma reductionStep_only_makes_smaller :
 
 lemma reductionLoop_only_makes_smaller :
   "cont1 \<noteq> cont \<Longrightarrow>
-   reductionLoop env state cont wa pa = ContractQuiescent nwa npa nsta cont1 \<Longrightarrow>
+   reductionLoop reducedBefore env state cont wa pa = ContractQuiescent reducedAfter nwa npa nsta cont1 \<Longrightarrow>
    size cont1 < size cont"
-  apply (induction env state cont wa pa arbitrary:cont1 nwa npa nsta rule:reductionLoop.induct)
-  subgoal for env state contract warnings payments cont1 nwa npa nsta
-    apply (simp only:reductionLoop.simps[of env state contract warnings payments])
+  apply (induction reducedBefore env state cont wa pa arbitrary:cont1 reducedAfter nwa npa nsta rule:reductionLoop.induct)
+  subgoal for reducedBefore env state contract warnings payments cont1 reducedAfter nwa npa nsta
+    apply (simp only:reductionLoop.simps[of reducedBefore env state contract warnings payments])
     apply (cases "reduceContractStep env state contract")
     subgoal for warning effect newState ncontract
       apply (simp del:reduceContractStep.simps reductionLoop.simps)
@@ -528,7 +589,7 @@ lemma reductionLoop_only_makes_smaller :
 
 lemma reduceContractUntilQuiescent_only_makes_smaller :
   "cont1 \<noteq> cont \<Longrightarrow>
-   reduceContractUntilQuiescent env state cont = ContractQuiescent wa pa nsta cont1 \<Longrightarrow>
+   reduceContractUntilQuiescent env state cont = ContractQuiescent reducedAfter wa pa nsta cont1 \<Longrightarrow>
    size cont1 < size cont"
   apply (simp only:reduceContractUntilQuiescent.simps)
   by (simp add: reductionLoop_only_makes_smaller)
@@ -555,13 +616,13 @@ lemma applyInput_only_makes_smaller :
 
 lemma applyAllLoop_only_makes_smaller :
   "cont1 \<noteq> cont \<Longrightarrow>
-   applyAllLoop env sta cont c wa ef = ApplyAllSuccess cwa1 pa1 sta1 cont1 \<Longrightarrow> cont1 \<noteq> cont \<Longrightarrow> size cont1 < size cont"
-  apply (induction env sta cont c wa ef rule:applyAllLoop.induct)
-  subgoal for env state contract inputs warnings payments
-    apply (simp only:applyAllLoop.simps[of env state contract inputs warnings payments])
+   applyAllLoop reducedBefore env sta cont c wa ef = ApplyAllSuccess reducedAfter cwa1 pa1 sta1 cont1 \<Longrightarrow> cont1 \<noteq> cont \<Longrightarrow> size cont1 < size cont"
+  apply (induction reducedBefore env sta cont c wa ef rule:applyAllLoop.induct)
+  subgoal for reducedBefore env state contract inputs warnings payments
+    apply (simp only:applyAllLoop.simps[of reducedBefore env state contract inputs warnings payments])
     apply (cases "reduceContractUntilQuiescent env state contract")
     apply (simp only:ReduceResult.case)
-    subgoal for wa pa nsta cont1
+    subgoal for reducedAfter wa pa nsta cont1
       apply (cases inputs)
       apply (simp only:list.case)
       apply (simp add:reduceContractUntilQuiescent_only_makes_smaller)
@@ -577,22 +638,22 @@ lemma applyAllLoop_only_makes_smaller :
   done
 
 lemma applyAllInputs_only_makes_smaller :
-  "applyAllInputs env sta cont c = ApplyAllSuccess cwa1 pa1 sta1 cont1 \<Longrightarrow>
+  "applyAllInputs env sta cont c = ApplyAllSuccess reducedAfter cwa1 pa1 sta1 cont1 \<Longrightarrow>
    cont1 \<noteq> cont \<Longrightarrow> size cont1 < size cont"
   apply (simp only:applyAllInputs.simps)
   using applyAllLoop_only_makes_smaller by blast
 
 lemma applyAllLoop_longer_doesnt_grow :
-  "applyAllLoop env sta cont h wa pa = ApplyAllSuccess cwa1 pa1 sta1 cont1 \<Longrightarrow>
-   applyAllLoop env sta cont (h @ t) wa pa = ApplyAllSuccess cwa2 pa2 sta2 cont2 \<Longrightarrow> size cont2 \<le> size cont1"
-  apply (induction h arbitrary: env sta cont t wa pa cwa1 pa1 sta1 cont1 cwa2 pa2 sta2 cont2)
-  subgoal for env sta cont t wa pa cwa1 pa1 sta1 cont1 cwa2 pa2 sta2 cont2
+  "applyAllLoop reducedBefore env sta cont h wa pa = ApplyAllSuccess reducedAfter1 cwa1 pa1 sta1 cont1 \<Longrightarrow>
+   applyAllLoop reducedBefore env sta cont (h @ t) wa pa = ApplyAllSuccess reducedAfter2 cwa2 pa2 sta2 cont2 \<Longrightarrow> size cont2 \<le> size cont1"
+  apply (induction h arbitrary: reducedBefore env sta cont t wa pa reducedAfter1 cwa1 pa1 sta1 cont1 reducedAfter2 cwa2 pa2 sta2 cont2)
+  subgoal for reducedBefore env sta cont t wa pa reducedAfter1 cwa1 pa1 sta1 cont1 reducedAfter2 cwa2 pa2 sta2 cont2
   apply (subst (asm) applyAllLoop.simps)
-  apply (subst (asm) applyAllLoop.simps[of env sta cont "[] @ t"])
+  apply (subst (asm) applyAllLoop.simps[of reducedBefore env sta cont "[] @ t"])
   apply (cases "reduceContractUntilQuiescent env sta cont")   
   apply (simp only:ReduceResult.case)
   apply (simp only:list.case append_Nil)
-  subgoal for wa pa nsta ncont
+  subgoal for reducedAfter wa pa nsta ncont
     apply (cases t)
     apply (simp only:list.case)
     apply blast
@@ -604,13 +665,13 @@ lemma applyAllLoop_longer_doesnt_grow :
       by simp
     done
   by simp
-  subgoal for hh ht env sta cont t wa pa cwa1 pa1 sta1 cont1 cwa2 pa2 sta2 cont2
-  apply (subst (asm) applyAllLoop.simps[of env sta cont "(hh # ht)"])
-  apply (subst (asm) applyAllLoop.simps[of env sta cont "(hh # ht) @ t"])
+  subgoal for hh ht reducedBefore env sta cont t wa pa reducedAfter1 cwa1 pa1 sta1 cont1 reducedAfter2 cwa2 pa2 sta2 cont2
+  apply (subst (asm) applyAllLoop.simps[of reducedBefore env sta cont "(hh # ht)"])
+  apply (subst (asm) applyAllLoop.simps[of reducedBefore env sta cont "(hh # ht) @ t"])
   apply (cases "reduceContractUntilQuiescent env sta cont")
   apply (simp only:ReduceResult.case List.append.append_Cons)
   apply (simp only:list.case)
-  subgoal for wa pa nsta ncont
+  subgoal for reducedAfter wa pa nsta ncont
     apply (cases "applyInput env nsta hh ncont")
     apply (simp only:ApplyResult.case)
     by simp
@@ -618,33 +679,34 @@ lemma applyAllLoop_longer_doesnt_grow :
   done
 
 lemma applyAllInputs_longer_doesnt_grow :
-  "applyAllInputs env sta cont h = ApplyAllSuccess cwa1 pa1 sta1 cont1 \<Longrightarrow>
-   applyAllInputs env sta cont (h @ t) = ApplyAllSuccess cwa2 pa2 sta2 cont2 \<Longrightarrow>
+  "applyAllInputs env sta cont h = ApplyAllSuccess reducedAfter1 cwa1 pa1 sta1 cont1 \<Longrightarrow>
+   applyAllInputs env sta cont (h @ t) = ApplyAllSuccess reducedAfter2 cwa2 pa2 sta2 cont2 \<Longrightarrow>
    size cont2 \<le> size cont1"
   apply (simp only:applyAllInputs.simps)
   by (simp add: applyAllLoop_longer_doesnt_grow)
 
 lemma applyAllInputs_once_modified_always_modified :
-  "applyAllInputs env sta cont [h] = ApplyAllSuccess cwa1 pa1 sta1 cont1 \<Longrightarrow>
+  "applyAllInputs env sta cont [h] = ApplyAllSuccess reducedAfter1 cwa1 pa1 sta1 cont1 \<Longrightarrow>
    cont1 \<noteq> cont \<Longrightarrow>
-   applyAllInputs env sta cont (h # t) = ApplyAllSuccess cwa2 pa2 sta2 cont2 \<Longrightarrow>
+   applyAllInputs env sta cont (h # t) = ApplyAllSuccess reducedAfter2 cwa2 pa2 sta2 cont2 \<Longrightarrow>
    cont2 \<noteq> cont"
   apply (rule smallerSize_implies_different)
   by (metis append_Cons append_Nil applyAllInputs.simps applyAllLoop_longer_doesnt_grow applyAllLoop_only_makes_smaller not_le)
 
+
 lemma computeTransactionIterative_aux :
   "fixInterval inte osta = IntervalTrimmed env sta \<Longrightarrow>
-   applyAllInputs env sta cont [h] = ApplyAllSuccess wa pa tsta ncont \<Longrightarrow>
+   applyAllInputs env sta cont [h] = ApplyAllSuccess reducedAfter wa pa tsta ncont \<Longrightarrow>
    fixInterval inte tsta = IntervalTrimmed nenv nsta \<Longrightarrow>
-   applyAllInputs nenv nsta ncont t = ApplyAllSuccess nwa npa fsta fcont \<Longrightarrow>
-   applyAllInputs env sta cont (h # t) = ApplyAllSuccess (wa @ nwa) (pa @ npa) fsta fcont"
-  using applyAllIterative2 fixIntervalIdempotentThroughApplyAllInputs2 by auto
+   applyAllInputs nenv nsta ncont t = ApplyAllSuccess reducedAfter2 nwa npa fsta fcont \<Longrightarrow>
+   applyAllInputs env sta cont (h # t) = ApplyAllSuccess True (wa @ nwa) (pa @ npa) fsta fcont"
+  using applyAllIterative2 fixIntervalIdempotentThroughApplyAllInputs by auto
 
 lemma computeTransactionIterative_aux2 :
   "fixInterval inte sta = IntervalTrimmed fIenv1 fIsta1 \<Longrightarrow>
-   applyAllInputs fIenv1 fIsta1 con [h] = ApplyAllSuccess cwa1 pa1 sta1 cont1 \<Longrightarrow>
+   applyAllInputs fIenv1 fIsta1 con [h] = ApplyAllSuccess reducedAfter1 cwa1 pa1 sta1 cont1 \<Longrightarrow>
     \<not> (cont1 = con \<and> (con \<noteq> Close \<or> accounts sta = [])) \<Longrightarrow>
-   applyAllInputs fIenv1 fIsta1 con (h # t) = ApplyAllSuccess cwa3 pa3 sta3 cont3 \<Longrightarrow>
+   applyAllInputs fIenv1 fIsta1 con (h # t) = ApplyAllSuccess reducedAfter3 cwa3 pa3 sta3 cont3 \<Longrightarrow>
     \<not> (cont3 = con \<and> (con \<noteq> Close \<or> accounts sta = []))"
   using applyAllInputs_once_modified_always_modified by blast
 
@@ -670,8 +732,8 @@ lemma computeTransactionIterative :
     apply (simp only:IntervalResult.case Let_def)
     apply (cases "applyAllInputs fIenv1 fIsta1 cont (inputs \<lparr>interval = inte, inputs = [h]\<rparr>)")
     apply (simp only:ApplyAllResult.case)
-    subgoal for cwa1 pa1 sta1 con1
-      apply (cases "cont = con1 \<and> (cont \<noteq> Close \<or> accounts sta = [])")
+    subgoal for reducedAfter1 cwa1 pa1 sta1 con1
+      apply (cases "\<not> reducedAfter1 \<and> (cont \<noteq> Close \<or> accounts sta = [])")
       apply simp
       apply (simp only:if_False)
       apply (cases "fixInterval (interval \<lparr>interval = inte, inputs = t\<rparr>) nsta")
@@ -679,8 +741,8 @@ lemma computeTransactionIterative :
       subgoal for fIenv2 fIsta2
         apply (cases "applyAllInputs fIenv2 fIsta2 ncont (inputs \<lparr>interval = inte, inputs = t\<rparr>)")
         apply (simp only:ApplyAllResult.case)
-        subgoal for cwa2 pa2 sta2 con2
-          apply (cases "ncont = con2 \<and> (ncont \<noteq> Close \<or> accounts nsta = [])")
+        subgoal for reducedAfter2 cwa2 pa2 sta2 con2
+          apply (cases "\<not> reducedAfter2 \<and> (ncont \<noteq> Close \<or> accounts nsta = [])")
           apply simp
           apply (simp only:if_False)
           apply (cases "fixInterval (interval \<lparr>interval = inte, inputs = h # t\<rparr>) sta")
@@ -688,15 +750,18 @@ lemma computeTransactionIterative :
           subgoal for fIenv3 fIsta3
             apply (cases "applyAllInputs fIenv3 fIsta3 cont (inputs \<lparr>interval = inte, inputs = h # t\<rparr>)")
             apply (simp only:ApplyAllResult.case)
-            subgoal for cwa3 pa3 sta3 con3
-              apply (cases "(cont = con3) \<and> (cont \<noteq> Close \<or> accounts sta = [])")
-              apply (metis IntervalResult.inject(1) Transaction.select_convs(1) Transaction.select_convs(2) computeTransactionIterative_aux2)
+            subgoal for reducedAfter3 cwa3 pa3 sta3 con3
+              apply (cases "\<not> reducedAfter3 \<and> (cont \<noteq> Close \<or> accounts sta = [])")
+              using applyAllIterative2 fixIntervalIdempotentThroughApplyAllInputs apply auto[1]
               apply (simp only:if_False)
-              by (metis ApplyAllResult.inject IntervalResult.inject(1) Transaction.select_convs(1) Transaction.select_convs(2) TransactionOutput.inject(1) TransactionOutputRecord.ext_inject applyAllInputs.simps applyLoopIdempotent2 fixIntervalIdempotentThroughApplyAllInputs)
-            apply (metis (no_types, lifting) ApplyAllResult.distinct(1) IntervalResult.inject(1) Transaction.select_convs(1) Transaction.select_convs(2) TransactionOutput.inject(1) TransactionOutputRecord.ext_inject computeTransactionIterative_aux)
-            by (metis (no_types, lifting) ApplyAllResult.distinct(3) IntervalResult.inject(1) Transaction.select_convs(1) Transaction.select_convs(2) TransactionOutput.inject(1) TransactionOutputRecord.ext_inject computeTransactionIterative_aux)
+              by (smt ApplyAllResult.inject IntervalResult.inject(1) Transaction.select_convs(1) Transaction.select_convs(2) TransactionOutput.inject(1) TransactionOutputRecord.ext_inject applyAllIterative applyAllPrefix1 applyAllPrefix2 fixIntervalIdempotentThroughApplyAllInputs)
+             apply (simp only:ApplyAllResult.case)
+            apply (smt ApplyAllResult.distinct(1) IntervalResult.inject(1) Transaction.select_convs(1) Transaction.select_convs(2) TransactionOutput.inject(1) TransactionOutputRecord.ext_inject applyAllIterative2 fixIntervalIdempotentThroughApplyAllInputs)
+            apply (simp only:ApplyAllResult.case)
+            by (smt ApplyAllResult.distinct(3) IntervalResult.inject(1) Transaction.select_convs(1) Transaction.select_convs(2) TransactionOutput.inject(1) TransactionOutputRecord.ext_inject applyAllIterative2 fixIntervalIdempotentThroughApplyAllInputs)
           by simp
-        by simp_all
+         apply simp
+        by simp
       by simp
     by simp_all
   by simp
@@ -721,13 +786,13 @@ lemma applyInput_reducesContract :
 
 lemma computeTransactionEquivalence_aux3 :
   "rest \<noteq> [] \<Longrightarrow>
-   applyAllInputs fIenv3 fIsta1 con [head] = ApplyAllSuccess iwa ipa fIsta3 con3 \<Longrightarrow>
-   \<not> applyAllInputs fIenv3 fIsta1 con (head # rest) = ApplyAllSuccess fwa fpa sta3 con3"
+   applyAllInputs fIenv3 fIsta1 con [head] = ApplyAllSuccess iReducedAfter iwa ipa fIsta3 con3 \<Longrightarrow>
+   \<not> applyAllInputs fIenv3 fIsta1 con (head # rest) = ApplyAllSuccess iReducedAfter2 fwa fpa sta3 con3"
   apply (simp only:applyAllInputs.simps)
-  apply (simp only:applyAllLoop.simps[of fIenv3 fIsta1])
+  apply (simp only:applyAllLoop.simps[of False fIenv3 fIsta1])
   apply (cases "reduceContractUntilQuiescent fIenv3 fIsta1 con")
   apply (simp only:ReduceResult.case list.case)
-  subgoal for reduceWarns pays curState cont
+  subgoal for reduceReduced reduceWarns pays curState cont
     apply (cases "applyInput fIenv3 curState head cont")
     subgoal for applyWarn newState cont2
       apply (simp del:reduceContractUntilQuiescent.simps applyInput.simps applyAllLoop.simps)
@@ -735,9 +800,9 @@ lemma computeTransactionEquivalence_aux3 :
       apply blast
       subgoal for head tail
         apply (simp del:reduceContractUntilQuiescent.simps applyInput.simps applyAllLoop.simps)
-        apply (simp only:applyAllLoop.simps[of fIenv3 newState])
+        apply (simp only:applyAllLoop.simps[of True fIenv3 newState])
         apply (cases "reduceContractUntilQuiescent fIenv3 newState cont2")
-        subgoal for reduceWarnsa paysa curState2 cont3
+        subgoal for reduceReduceda reduceWarnsa paysa curState2 cont3
           apply (simp only:ReduceResult.case list.case)
           apply (cases "applyInput fIenv3 curState2 head cont3")
           apply (simp only:ApplyResult.case)
@@ -748,6 +813,10 @@ lemma computeTransactionEquivalence_aux3 :
       done
       by simp
     by simp
+
+lemma notFalseAndTrue : "\<not> False \<and> True = True"
+  by simp
+
 
 lemma computeTransactionStepEquivalence :
   "rest \<noteq> [] \<Longrightarrow>
@@ -773,31 +842,34 @@ lemma computeTransactionStepEquivalence :
     apply (simp del:fixInterval.simps computeTransaction.simps applyAllInputs.simps)
     apply (cases "applyAllInputs fIenv1 fIsta1 con [head]")
       apply (simp only:ApplyAllResult.case)
-      subgoal for cwa1 pa1 sta1 con1
-        apply (cases "con = con1 \<and> (con \<noteq> Close \<or> accounts sta = [])")
-        apply (simp del:fixInterval.simps computeTransaction.simps applyAllInputs.simps)
+    subgoal for reducedAfter1 cwa1 pa1 sta1 con1
+        apply (cases "\<not> reducedAfter1 \<and> (con \<noteq> Close \<or> accounts sta = [])")
+        apply simp
+        apply (simp del:fixInterval.simps computeTransaction.simps applyAllInputs.simps only:refl if_False)
         apply (cases "fixInterval interv ista2")
         subgoal for fIenv2 fIsta2
           apply (cases "applyAllInputs fIenv1 fIsta1 con (head # rest)")
           apply (simp only:ApplyAllResult.case if_False)
-          subgoal for cwa2 pa2 sta2 con2
-            apply (cases "con = con2 \<and> (con \<noteq> Close \<or> accounts sta = [])")
+          subgoal for reducedAfter2 cwa2 pa2 sta2 con2
+            apply (cases "\<not> reducedAfter2 \<and> (con \<noteq> Close \<or> accounts sta = [])")
             apply simp
-            apply (simp only:if_False)
+            apply (simp del:fixInterval.simps computeTransaction.simps applyAllInputs.simps only:refl if_False)
             apply (cases "fixInterval interv ista")
             apply (simp only:IntervalResult.case Let_def)
             subgoal for fIenv3 fIsta3
               apply (cases "applyAllInputs fIenv3 fIsta3 icont rest")
               apply (simp only:ApplyAllResult.case) 
-              subgoal for cwa3 pa3 sta3 con3
-                apply (cases "icont = con3 \<and> (icont \<noteq> Close \<or> accounts ista = [])")
-                apply (simp only:bool.case refl if_True)
-                 apply (metis IntervalResult.inject(1) TransactionOutput.inject(1) TransactionOutputRecord.ext_inject applyAllInputs.simps applyLoopIdempotent2 computeTransactionEquivalence_aux3 fixIntervalIdempotentThroughApplyAllInputs)
+              subgoal for reducedAfter3 cwa3 pa3 sta3 con3
+                apply (cases "\<not> reducedAfter3 \<and> (icont \<noteq> Close \<or> accounts ista = [])")
+                 apply (simp del:fixInterval.simps computeTransaction.simps applyAllInputs.simps only:refl if_False)
+                apply (smt ApplyAllResult.inject IntervalResult.inject(1) TransactionOutput.inject(1) TransactionOutputRecord.ext_inject applyAllIterative fixIntervalIdempotentThroughApplyAllInputs)
                 using computeTransactionIterative_aux by auto
-               apply (metis (no_types, lifting) ApplyAllResult.simps(3) IntervalResult.inject(1) TransactionOutput.inject(1) TransactionOutputRecord.ext_inject applyAllInputs.simps applyAllPrefix1 applyAllPrefix2 applyLoopIdempotent fixIntervalIdempotentThroughApplyAllInputs2)
-               by (metis (no_types, lifting) ApplyAllResult.simps(5) IntervalResult.inject(1) TransactionOutput.inject(1) TransactionOutputRecord.ext_inject applyAllInputs.simps applyAllPrefix1 applyAllPrefix2 applyLoopIdempotent fixIntervalIdempotentThroughApplyAllInputs2)
-             by (simp add: fixIntervalIdempotentThroughApplyAllInputs)
-            apply simp
+               apply (simp only:ApplyAllResult.case)
+              apply (metis ApplyAllResult.distinct(1) IntervalResult.inject(1) TransactionOutput.inject(1) TransactionOutputRecord.ext_inject applyAllIterative fixIntervalIdempotentThroughApplyAllInputs)
+               apply (simp only:ApplyAllResult.case)
+              by (metis ApplyAllResult.distinct(3) IntervalResult.inject(1) TransactionOutput.inject(1) TransactionOutputRecord.ext_inject applyAllIterative fixIntervalIdempotentThroughApplyAllInputs)
+            by (simp add: fixIntervalIdempotentThroughApplyAllInputs)
+          apply simp
            by simp
          subgoal for err2
            apply (cases "applyAllInputs fIenv1 fIsta1 con (head # rest)")
@@ -814,14 +886,14 @@ lemma applyAllInputs_prefix_error :
   "a = ApplyAllAmbiguousSlotIntervalError \<or> a = ApplyAllNoMatchError \<Longrightarrow>
    applyAllInputs env fixSta txOutCont [head] = a \<Longrightarrow>
    applyAllInputs env fixSta txOutCont (head # tail) = a"
-  apply (simp only:applyAllInputs.simps applyAllLoop.simps[of env fixSta txOutCont])
+  apply (simp only:applyAllInputs.simps applyAllLoop.simps[of False env fixSta txOutCont])
   apply (cases "reduceContractUntilQuiescent env fixSta txOutCont")
-  subgoal for reduceWarns pays curState cont
+  subgoal for reduceReduced reduceWarns pays curState cont
     apply (simp only:ReduceResult.case list.case)
     apply (cases "applyInput env curState head cont")
     subgoal for applyWarn newState cont2
       apply (simp only:ApplyResult.case)
-      apply (simp only:applyAllLoop.simps[of env newState cont2])
+      apply (simp only:applyAllLoop.simps[of True env newState cont2])
       apply (cases "reduceContractUntilQuiescent env newState cont2")
       subgoal for reduceWarns3 pays3 curState3 cont3
         apply (simp only:ReduceResult.case list.case)
@@ -830,35 +902,26 @@ lemma applyAllInputs_prefix_error :
     by simp
   by simp
 
-lemma applyInput_success_changes_contract :
-  "applyInput env reduceState head txOutCont = Applied applyWarn applyState applyCont \<Longrightarrow> txOutCont \<noteq> applyCont"
-  apply (cases txOutCont)
-  apply simp_all
-  subgoal for caselist timeout contract
-    using applyCases_only_makes_smaller by fastforce
-  done
 
 lemma applyAllInputs_noEmpty_changes_contract :
- "applyAllInputs env fixSta txOutCont (head # []) = ApplyAllSuccess warnings payments newState cont \<Longrightarrow>
-  txOutCont \<noteq> cont"
+ "applyAllInputs env fixSta txOutCont (head # []) = ApplyAllSuccess reduced warnings payments newState cont \<Longrightarrow>
+  reduced"
   apply (simp del:reduceContractUntilQuiescent.simps)
   apply (cases "reduceContractUntilQuiescent env fixSta txOutCont")
-  subgoal for reduceWarns reducePays reduceState reduceCont
+  subgoal for reduceReduced reduceWarns reducePays reduceState reduceCont
   apply (simp only:ReduceResult.case list.case)
     apply (cases "reduceCont = txOutCont")
     apply (cases "applyInput env reduceState head reduceCont")
     subgoal for applyWarn applyState applyCont
       apply (simp only:ApplyResult.case)
-      by (metis applyAllLoop_only_makes_smaller applyInput_only_makes_smaller applyInput_success_changes_contract not_less_iff_gr_or_eq)
+      using applyAllLoop_preserves_reduced by blast
      apply simp
     apply (cases "applyInput env reduceState head reduceCont")
     subgoal for applyWarn applyState applyCont
       apply (simp only:ApplyResult.case)
-      apply (drule reduceContractUntilQuiescent_only_makes_smaller[of reduceCont txOutCont env fixSta reduceWarns reducePays reduceState])
+      apply (drule reduceContractUntilQuiescent_only_makes_smaller[of reduceCont txOutCont env fixSta reduceReduced reduceWarns reducePays reduceState])
        apply simp
-      apply (rule not_sym)
-      apply (rule smallerSize_implies_different)
-      by (metis applyAllLoop_only_makes_smaller applyInput_only_makes_smaller dual_order.strict_trans)
+      using applyAllLoop_preserves_reduced by blast
     by simp
   by simp
 
@@ -870,19 +933,20 @@ lemma computeTransaction_prefix_error :
   subgoal for env fixSta
   apply (simp only:IntervalResult.case Let_def)
     apply (cases "applyAllInputs env fixSta txOutCont [head]")
-    subgoal for warnings payments newState cont
+    subgoal for reduced warnings payments newState cont
       apply (simp only:ApplyAllResult.case)
     apply (cases "applyAllInputs env fixSta txOutCont (head # tail)")
-    subgoal for warnings2 payments2 newState2 cont2
+    subgoal for reduced2 warnings2 payments2 newState2 cont2
       apply (simp only:ApplyAllResult.case)
-      apply (cases "txOutCont = cont \<and> (txOutCont \<noteq> Close \<or> accounts txOutStat = [])")
-      apply (cases "txOutCont = cont2 \<and> (txOutCont \<noteq> Close \<or> accounts txOutStat = [])")
+      apply (cases "\<not> reduced \<and> (txOutCont \<noteq> Close \<or> accounts txOutStat = [])")
+      apply (cases "\<not> reduced2 \<and> (txOutCont \<noteq> Close \<or> accounts txOutStat = [])")
       apply simp
-    apply (simp only:if_False)
+      apply (simp only:if_True bool_simps)
     using applyAllInputs_noEmpty_changes_contract apply blast
     by auto
-   apply (simp add: applyAllInputs_noEmpty_changes_contract)
-  by (simp add: applyAllInputs_noEmpty_changes_contract)
+  apply (simp only:ApplyAllResult.case)
+  using applyAllInputs_noEmpty_changes_contract apply fastforce
+  using applyAllInputs_noEmpty_changes_contract by fastforce
   apply (metis (no_types, lifting) applyAllInputs_prefix_error)
   by (metis (no_types, lifting) applyAllInputs_prefix_error)
   by simp
@@ -891,11 +955,6 @@ lemma fixInterval_doesnt_care_about_inputs :
   "fixInterval (interval \<lparr>interval = interv, inputs = inp1\<rparr>) sta = IntervalTrimmed env fixSta \<Longrightarrow>
    fixInterval (interval \<lparr>interval = interv, inputs = inp2\<rparr>) sta = IntervalTrimmed env fixSta"
   by simp
-
-lemma reduceContractUntilQuiescent_idempotent :
-  "reduceContractUntilQuiescent env newState cont2 = ContractQuiescent reduceWarns2 pays2 ista icont \<Longrightarrow>
-   reduceContractUntilQuiescent env ista icont = ContractQuiescent [] [] ista icont"
-  using reductionLoopIdempotent by auto
 
 lemma fixInterval_idemp_on_same_minSlot :
   "fixInterval interv sta = IntervalTrimmed env fixSta \<Longrightarrow>
@@ -909,29 +968,29 @@ lemma fixInterval_idemp_on_same_minSlot :
 
 lemma fixInterval_idemp_after_computeTransaction :
   "fixInterval interv sta = IntervalTrimmed env fixSta \<Longrightarrow>
-   reduceContractUntilQuiescent env fixSta con = ContractQuiescent reduceWarns pays curState cont \<Longrightarrow>
+   reduceContractUntilQuiescent env fixSta con = ContractQuiescent reduceReduced reduceWarns pays curState cont \<Longrightarrow>
    applyInput env curState head cont = Applied applyWarn newState cont2 \<Longrightarrow>
-   reduceContractUntilQuiescent env newState cont2 = ContractQuiescent reduceWarns2 pays2 ista icont \<Longrightarrow>
+   reduceContractUntilQuiescent env newState cont2 = ContractQuiescent reduceReduced2 reduceWarns2 pays2 ista icont \<Longrightarrow>
    fixInterval interv ista = IntervalTrimmed env ista"
   by (simp add: applyInput_preserves_minSlot fixInterval_idemp_on_same_minSlot reductionLoop_preserves_minSlot)
 
 lemma applyAllLoop_independet_of_acc_error1 :
-  "applyAllLoop env sta cont htail wa pa = ApplyAllNoMatchError \<Longrightarrow>
-   applyAllLoop env sta cont htail wa2 pa2 = ApplyAllNoMatchError"
-  apply (induction htail arbitrary: env sta cont wa pa wa2 pa2)
+  "applyAllLoop reducedBefore env sta cont htail wa pa = ApplyAllNoMatchError \<Longrightarrow>
+   applyAllLoop reducedBefore env sta cont htail wa2 pa2 = ApplyAllNoMatchError"
+  apply (induction htail arbitrary: reducedBefore env sta cont wa pa wa2 pa2)
   apply (force split:ReduceResult.split)
-  subgoal for head tail env sta cont wa pa wa2 pa2
-    apply (simp only:applyAllLoop.simps[of env sta cont "head # tail"])
+  subgoal for head tail reducedBefore env sta cont wa pa wa2 pa2
+    apply (simp only:applyAllLoop.simps[of reducedBefore env sta cont "head # tail"])
     by (auto split:ReduceResult.split ApplyResult.split simp del:applyAllLoop.simps)
   done
 
 lemma applyAllLoop_independet_of_acc_error2 :
-  "applyAllLoop env sta cont htail wa pa = ApplyAllAmbiguousSlotIntervalError \<Longrightarrow>
-   applyAllLoop env sta cont htail wa2 pa2 = ApplyAllAmbiguousSlotIntervalError"
-  apply (induction htail arbitrary: env sta cont wa pa wa2 pa2)
+  "applyAllLoop reducedBefore env sta cont htail wa pa = ApplyAllAmbiguousSlotIntervalError \<Longrightarrow>
+   applyAllLoop reducedBefore env sta cont htail wa2 pa2 = ApplyAllAmbiguousSlotIntervalError"
+  apply (induction htail arbitrary: reducedBefore env sta cont wa pa wa2 pa2)
   apply (force split:ReduceResult.split)
-  subgoal for head tail env sta cont wa pa wa2 pa2
-    apply (simp only:applyAllLoop.simps[of env sta cont "head # tail"])
+  subgoal for head tail reducedBefore env sta cont wa pa wa2 pa2
+    apply (simp only:applyAllLoop.simps[of reducedBefore env sta cont "head # tail"])
     by (auto split:ReduceResult.split ApplyResult.split simp del:applyAllLoop.simps)
   done
 
@@ -956,38 +1015,45 @@ lemma computeTransactionStepEquivalence_error :
       apply (subst (asm) fixInterval_doesnt_care_about_inputs[of interv "[head]" sta env fixSta "head # hrest # htail"])
       apply blast
       apply (simp only:IntervalResult.case)
-      apply (simp only:applyAllInputs.simps applyAllLoop.simps[of env fixSta])
+      apply (simp only:applyAllInputs.simps applyAllLoop.simps[of True env fixSta])
       apply (cases "reduceContractUntilQuiescent env fixSta con")
-      subgoal for reduceWarns pays curState cont
+      subgoal for reducedBefore reduceWarns pays curState cont
         apply (simp del:fixInterval.simps reduceContractUntilQuiescent.simps computeTransaction.simps applyInput.simps)
         apply (cases "applyInput env curState head cont")
         subgoal for applyWarn newState cont2
           apply (simp only:ApplyResult.case)
-          apply (simp only:applyAllInputs.simps applyAllLoop.simps[of env newState] computeTransaction.simps Let_def)
+          apply (simp only:applyAllInputs.simps applyAllLoop.simps[of True env newState] computeTransaction.simps Let_def)
           apply (cases "reduceContractUntilQuiescent env newState cont2")
-          subgoal for reduceWarns2 pays2 curState2 cont3
+          subgoal for reducedBefore2 reduceWarns2 pays2 curState2 cont3
             apply (simp only:ReduceResult.case list.case ApplyAllResult.case)
             apply (cases "con = cont3")
             apply (metis applyInput_reducesContract dual_order.strict_trans order.asym reduceContractUntilQuiescent_only_makes_smaller)
             apply (simp del:fixInterval.simps reduceContractUntilQuiescent.simps computeTransaction.simps applyInput.simps)
 
-            apply (simp only:fixInterval_idemp_after_computeTransaction[of interv sta env fixSta con
+            apply (simp only:fixInterval_idemp_after_computeTransaction[of interv sta env fixSta con reducedBefore
                                                                            reduceWarns pays curState cont
-                                                                           head applyWarn newState cont2
+                                                                           head applyWarn newState cont2 reducedBefore2
                                                                            reduceWarns2 pays2 ista icont])
-            apply (simp only:IntervalResult.case applyAllLoop.simps[of env ista icont])
-            apply (simp only:reduceContractUntilQuiescent_idempotent ReduceResult.case Transaction.select_convs list.case)
+            apply (simp only:IntervalResult.case applyAllLoop.simps[of True env ista icont])
+            apply (simp only:reduceContractUntilQuiescentIdempotent ReduceResult.case Transaction.select_convs list.case)
             apply (cases "applyInput env ista hrest icont")
             subgoal for applyWarna newState2 cont4
               apply (simp only:ApplyResult.case)
-              apply (cases "applyAllLoop env newState2 cont4 htail
+              apply (cases "applyAllLoop True env newState2 cont4 htail
                                          (([] @ convertReduceWarnings reduceWarns @ convertApplyWarning applyWarn) @
                                           convertReduceWarnings reduceWarns2 @ convertApplyWarning applyWarna)
                                          (([] @ pays) @ pays2)")
-              apply (smt ApplyAllResult.simps(8) TransactionOutput.distinct(1) applyAllLoop_only_makes_smaller applyInput_reducesContract dual_order.strict_trans reduceContractUntilQuiescent_only_makes_smaller smallerSize_implies_different)
-              using applyAllLoop_independet_of_acc_error1 apply auto[1]
-              using applyAllLoop_independet_of_acc_error2 by auto
-            by simp
+                apply (simp only:ApplyAllResult.case)
+              subgoal for x11 x12 x13 x14 x15
+                apply (cases "\<not> x11 \<and> (con \<noteq> Close \<or> accounts sta = [])")
+                 apply (simp only:if_True)
+                apply (rule mp[of "applyAllLoop True env newState2 cont4 htail ((([] @ convertReduceWarnings reduceWarns @ convertApplyWarning applyWarn) @ convertReduceWarnings reduceWarns2 @ convertApplyWarning applyWarna) @ []) ((([] @ pays) @ pays2) @ []) = ApplyAllSuccess False x12 x13 x14 x15"])
+                  apply (smt ApplyAllResult.simps(8) ApplyResult.distinct(1) ApplyResult.simps(4) ReduceResult.simps(4) append.assoc append_self_conv applyAllInputsPrefix1 applyAllInputsPrefix2 applyAllLoop.simps applyAllLoopJustAppendsWarningsAndEffects applyInput.simps(2) list.simps(5) reduceContractUntilQuiescentIdempotent)
+                 apply simp
+                by auto
+               apply (metis (no_types, lifting) ApplyAllResult.simps(9) ApplyResult.simps(4) ReduceResult.simps(4) applyAllLoop.simps applyAllLoop_independet_of_acc_error1 list.simps(5) reduceContractUntilQuiescentIdempotent)
+              by (metis (no_types, lifting) ApplyAllResult.simps(10) ApplyResult.simps(4) ReduceResult.simps(4) applyAllLoop.simps applyAllLoop_independet_of_acc_error2 list.simps(5) reduceContractUntilQuiescentIdempotent)
+            using reduceContractUntilQuiescentIdempotent by auto
           by simp
         by simp
       by simp
@@ -1077,6 +1143,7 @@ lemma playTraceAuxToSingleInputIsEquivalent_induction_step_aux :
           apply (simp del:computeTransaction.simps playTraceAux.simps)
           subgoal premises facts
             apply(subst facts(1)[symmetric])
+            thm facts
             apply (simp only:playTraceAux.simps Let_def)
             apply (subst computeTransactionStepEquivalence_error)
             apply simp
